Include phantom parameter in fset definition.

theories/fset.v
@@ -51,12 +51,10 @@ Variables (T : ordType).
 
 Local Open Scope ord_scope.
 
-CoInductive fset_type := FSet {
+CoInductive fset_type (p : phant T) := FSet {
   fsval : seq T;
   _ : sorted (@Ord.lt T) fsval
 }.
-Definition fset_of of phant T := fset_type.
-Identity Coercion type_of_fset_of : fset_of >-> fset_type.
 
 Lemma fset_subproof (s : seq T) :
   sorted (@Ord.lt T) (sort (@Ord.leq T) (undup s)).
@@ -73,19 +71,23 @@ End Def.
 
 Module Exports.
 
-Notation "{ 'fset' T }" := (@fset_of _ (Phant T))
+Notation "{ 'fset' T }" := (@fset_type _ (Phant T))
   (at level 0, format "{ 'fset'  T }") : type_scope.
 Coercion fsval : fset_type >-> seq.
-Canonical fset_subType T := [subType for @fsval T].
-Definition fset_eqMixin T := [eqMixin of fset_type T by <:].
-Canonical fset_eqType T :=
-  Eval hnf in EqType (fset_type T) (fset_eqMixin T).
-Definition fset_choiceMixin T := [choiceMixin of fset_type T by <:].
-Canonical fset_choiceType T :=
-  Eval hnf in ChoiceType (fset_type T) (fset_choiceMixin T).
-Definition fset_ordMixin T := [ordMixin of fset_type T by <:].
-Canonical fset_ordType T :=
-  Eval hnf in OrdType (fset_type T) (fset_ordMixin T).
+
+Section Instances.
+
+Variable T : ordType.
+
+Canonical fset_subType := [subType for @fsval _ (Phant T)].
+Definition fset_eqMixin := [eqMixin of {fset T} by <:].
+Canonical fset_eqType := Eval hnf in EqType {fset T} fset_eqMixin.
+Definition fset_choiceMixin := [choiceMixin of {fset T} by <:].
+Canonical fset_choiceType := Eval hnf in ChoiceType {fset T} fset_choiceMixin.
+Definition fset_ordMixin := [ordMixin of {fset T} by <:].
+Canonical fset_ordType := Eval hnf in OrdType {fset T} fset_ordMixin.
+
+End Instances.
 
 End Exports.
 
@@ -95,25 +97,11 @@ Export FSet.Exports.
 
 Delimit Scope fset_scope with fset.
 
-Section ReExports.
-
-(** This redundancy is needed to make inference more robust when using
-    [fset_of] instead of [fset_type]. *)
-
-Variable T : ordType.
-
-Canonical fset_of_subType := Eval hnf in [subType of {fset T}].
-Canonical fset_of_eqType := Eval hnf in [eqType of {fset T}].
-Canonical fset_of_choiceType := Eval hnf in [choiceType of {fset T}].
-Canonical fset_of_ordType := Eval hnf in [ordType of {fset T}].
-
-End ReExports.
-
 Lemma fset_key : unit. Proof. exact: tt. Qed.
 Definition fset (T : ordType) : seq T -> {fset T} :=
   locked_with fset_key
               (fun (s : seq T) =>
-                 @FSet.FSet T _ (FSet.fset_subproof s)).
+                 @FSet.FSet T _ _ (FSet.fset_subproof s)).
 
 Prenex Implicits fset.
 
@@ -131,8 +119,8 @@ Proof. by rewrite [fset]unlock inE /= mem_sort mem_undup. Qed.
 
 Implicit Type s : {fset T}.
 
-Definition fset0 := @FSet.FSet T [::] erefl : {fset T}.
-Definition fset1 x := @FSet.FSet T [:: x] erefl : {fset T}.
+Definition fset0 := @FSet.FSet T _ [::] erefl : {fset T}.
+Definition fset1 x := @FSet.FSet T _ [:: x] erefl : {fset T}.
 Definition fsetU s1 s2 := fset (val s1 ++ val s2).
 Definition fset_filter P s := fset [seq x <- s | P x].
 Definition fsetI s1 s2 := fset_filter (mem s1) s2.
@@ -238,7 +226,7 @@ Lemma fsetP s : fset_spec s.
 Proof.
 case: s=> [[|x xs] /= Pxs]; first by rewrite eq_axiomK; apply: FSetSpec0.
 have Pxs' := path_sorted Pxs.
-set s' : {fset T} := FSet.FSet Pxs'; set s : {fset T} := FSet.FSet _.
+set s' : {fset T} := FSet.FSet _ Pxs'; set s : {fset T} := FSet.FSet _ _.
 have x_nin_s : x \notin s'.
   apply/negP=> /(allP (order_path_min (@Ord.lt_trans T) Pxs)).
   by rewrite Ord.ltxx.
@@ -253,7 +241,7 @@ Lemma fset_rect (P : {fset T} -> Type) :
 Proof.
 move=> H0 HS []; elim=> [|/= x xs IH] Pxs; first by rewrite eq_axiomK.
 move: IH => /(_ (path_sorted Pxs)).
-set s : {fset T} := FSet.FSet _; set s' : {fset T} := FSet.FSet _ => Ps.
+set s : {fset T} := FSet.FSet _ _; set s' : {fset T} := FSet.FSet _ _ => Ps.
 have x_nin_s : x \notin s.
   apply/negP=> /(allP (order_path_min (@Ord.lt_trans T) Pxs)).
   by rewrite Ord.ltxx.
